\documentclass{article}

\usepackage{amsmath}
\begin{document}
	\section*{Change spacing in math-environement}
	\begin{equation*}
		\setlength{\jot}{10pt}
		\begin{aligned}
			&\left(1+\sum_{j=1}^{\infty}(-1)^j q^{\frac{j(3j-1)}{2}} (1+q^j)\right)
			\sum_{n=0}^{\infty}p(n)q^n=1\\
			%
			\Leftrightarrow&\left(-1+\sum_{j=0}^{\infty}(-1)^j q^{\frac{j(3j-1)}{2}} (1+q^j)\right)
			\sum_{n=0}^{\infty}p(n)q^n=1\\
			%
			\Leftrightarrow&\left(\sum_{j=0}^{\infty}(-1)^j q^{\frac{j(3j-1)}{2}} (1+q^j)\right)\left(\sum_{n=0}^{\infty}p(n)q^n=1\right)-1=\sum_{n=0}^{\infty}p(n)q^n\\
			%
			\Leftrightarrow&\left(\sum_{n=0}^{\infty}\sum_{j=0}^{n}(-1)^j q^{\frac{j(3j-1)}{2}}p(n-j)q^{n-j}\right)-1
			=\sum_{n=0}^{\infty}p(n)q^n\\
			%
			\Leftrightarrow&\phantom{\Biggl(}\sum_{n=1}^{\infty}\sum_{j=0}^{n}(-1)^j q^{\frac{j(3j-1)}{2}}p(n-j)q^{n-j}
			=\sum_{n=1}^{\infty}p(n)q^n
		\end{aligned}
	\end{equation*}
\end{document}